theories/Handlers/MQ.v
@@ -67,7 +67,7 @@ Section defs.
   | mq_produce_lost_msg : forall s pid val,
       mq_chain_rule s s (pid @ None <~ produce val).
 
-  Global Instance MQHandler : @Handler PID req_t ret_t :=
+  Global Instance t : @Handler PID req_t ret_t :=
     { h_state := S;
       h_chain_rule := mq_chain_rule;
     }.
